theories/typing/bool.v
@@ -26,7 +26,7 @@ Section typing.
 
   Lemma type_bool_instr (b : Datatypes.bool) : typed_val #b bool.
   Proof.
-    iIntros (E L tid) "_ _ $ $ _". iApply wp_value.
+    iIntros (E L tid ?) "_ _ $ $ _". iApply wp_value.
     rewrite tctx_interp_singleton tctx_hasty_val' //. by destruct b.
   Qed.
 
@@ -41,7 +41,7 @@ Section typing.
     typed_body E L C T e1 -∗ typed_body E L C T e2 -∗
     typed_body E L C T (if: p then e1 else e2).
   Proof.
-    iIntros (Hp) "He1 He2". iIntros (tid) "#LFT #HE Htl HL HC HT".
+    iIntros (Hp) "He1 He2". iIntros (tid qmax) "#LFT #HE Htl HL HC HT".
     iDestruct (big_sepL_elem_of _ _ _ Hp with "HT") as "#Hp".
     wp_bind p. iApply (wp_hasty with "Hp").
     iIntros ([[| |[|[]|]]|]) "_ H1"; try done; wp_case.
