theories/typing/int.v
@@ -26,7 +26,7 @@ Section typing.
 
   Lemma type_int_instr (z : Z) : typed_val #z int.
   Proof.
-    iIntros (E L tid) "_ _ $ $ _". iApply wp_value.
+    iIntros (E L tid ?) "_ _ $ $ _". iApply wp_value.
     by rewrite tctx_interp_singleton tctx_hasty_val' //.
   Qed.
 
@@ -39,7 +39,7 @@ Section typing.
   Lemma type_plus_instr E L p1 p2 :
     ⊢ typed_instruction_ty E L [p1 ◁ int; p2 ◁ int] (p1 + p2) int.
   Proof.
-    iIntros (tid) "_ _ $ $ [Hp1 [Hp2 _]]".
+    iIntros (tid ?) "_ _ $ $ [Hp1 [Hp2 _]]".
     wp_apply (wp_hasty with "Hp1"). iIntros ([[]|]) "_ H1"; try done.
     wp_apply (wp_hasty with "Hp2"). iIntros ([[]|]) "_ H2"; try done.
     wp_op. by rewrite tctx_interp_singleton tctx_hasty_val' //.
@@ -55,7 +55,7 @@ Section typing.
   Lemma type_minus_instr E L p1 p2 :
     ⊢ typed_instruction_ty E L [p1 ◁ int; p2 ◁ int] (p1 - p2) int.
   Proof.
-    iIntros (tid) "_ _ $ $ [Hp1 [Hp2 _]]".
+    iIntros (tid ?) "_ _ $ $ [Hp1 [Hp2 _]]".
     wp_apply (wp_hasty with "Hp1"). iIntros ([[]|]) "_ H1"; try done.
     wp_apply (wp_hasty with "Hp2"). iIntros ([[]|]) "_ H2"; try done.
     wp_op. by rewrite tctx_interp_singleton tctx_hasty_val' //.
@@ -71,7 +71,7 @@ Section typing.
   Lemma type_le_instr E L p1 p2 :
     ⊢ typed_instruction_ty E L [p1 ◁ int; p2 ◁ int] (p1 ≤ p2) bool.
   Proof.
-    iIntros (tid) "_ _ $ $ [Hp1 [Hp2 _]]".
+    iIntros (tid ?) "_ _ $ $ [Hp1 [Hp2 _]]".
     wp_apply (wp_hasty with "Hp1"). iIntros ([[]|]) "_ H1"; try done.
     wp_apply (wp_hasty with "Hp2"). iIntros ([[]|]) "_ H2"; try done.
     wp_op; case_bool_decide; by rewrite tctx_interp_singleton tctx_hasty_val' //.
