theories/typing/lib/diverging_static.v
@@ -27,19 +27,37 @@ Section diverging_static.
     intros Hf E L. iApply type_fn; [solve_typing..|]. iIntros "/= !#".
       iIntros (α ϝ ret arg). inv_vec arg=>x f. simpl_subst.
     iApply type_let; [apply Hf|solve_typing|]. iIntros (call); simpl_subst.
-    iApply (type_cont [_] [] (λ r, [(r!!!0%fin:val) ◁ box (unit)])).
-    { iIntros (k). simpl_subst.
-      iApply type_equivalize_lft_static.
-      iApply (type_call [ϝ] ()); solve_typing. }
-    iIntros "!# *". inv_vec args=>r. simpl_subst.
-    iApply (type_cont [] [] (λ r, [])).
-    { iIntros (kloop). simpl_subst. iApply type_jump; solve_typing. }
-    iIntros "!# *". inv_vec args. simpl_subst.
-    iApply type_jump; solve_typing.
+    (* Drop to Iris *)
+    iIntros (tid qmax) "#LFT #HE Hna HL Hk (Hcall & Hx & Hf & _)".
+    (* We need a ϝ token to show that we can call F despite it being non-'static. *)
+    iMod (lctx_lft_alive_tok ϝ with "HE HL") as (qϝ) "(Hϝ & HL & _)";
+      [solve_typing..|].
+    iMod (lctx_lft_alive_tok_noend α with "HE HL") as (q) "(Hα & _ & _)";
+      [solve_typing..|].
+    iMod (lft_eternalize with "Hα") as "#Hα".
+    iAssert (type_incl (box (&shr{α} T)) (box (&shr{static} T))) as "#[_ [Hincl _]]".
+    { iApply box_type_incl. iNext. iApply shr_type_incl; first done.
+      iApply type_incl_refl. }
+    wp_let. rewrite tctx_hasty_val.
+    iApply (type_call_iris _ [ϝ] () [_; _] with "LFT HE Hna [Hϝ] Hcall [Hx Hf]").
+    - solve_typing.
+    - by rewrite /= (right_id static).
+    - simpl. iFrame. iSplit; last done. rewrite !tctx_hasty_val.
+      iApply "Hincl". done.
+    - iClear "Hα Hincl". iIntros (r) "Htl Hϝ1 Hret". wp_rec.
+      (* Go back to the type system. *)
+      iApply (type_type _ [] _ [] with "[] LFT HE Htl [] Hk [-]"); last first.
+      { rewrite /tctx_interp /=. done. }
+      { rewrite /llctx_interp /=. done. }
+      iApply (type_cont [] [] (λ _, [])).
+      + iIntros (?). simpl_subst. iApply type_jump; solve_typing.
+      + iIntros "!#" (? args). inv_vec args. simpl_subst. iApply type_jump; solve_typing.
   Qed.
 
-  (** Variant of the above where the lifetime is in an arbitrary invariant
-      position.  This is incompatible with branding!
+
+  (** With the right typing rule, we can prove a variant of the above where the
+      lifetime is in an arbitrary invariant position, without even leaving the
+      type system.  This is incompatible with branding!
 
       Our [TyWf] is not working well for type constructors (we have no way of
       representing the fact that well-formedness is somewhat "uniform"), so we
@@ -49,8 +67,13 @@ Section diverging_static.
       list would require some induction-based reasoning principles that we do
       not have, but showing that it works for one lifetime is enough to
       demonstrate the principle). *)
-  Lemma diverging_static_loop_type' (T : lft → type) F κuser Euser call_once
+  Lemma diverging_static_loop_type_bad (T : lft → type) F κuser Euser call_once
         `{!TyWf F} :
+    (* The "bad" type_equivalize_lft_static rule *)
+    (∀ E L C T κ e,
+      (⊢ typed_body ((static ⊑ₑ κ) :: E) L C T e) →
+      ⊢ typed_body E ((κ ⊑ₗ []) :: L) C T e) →
+    (* Typing of this function *)
     let _ : (∀ κ, TyWf (T κ)) := λ κ, {| ty_lfts := [κ; κuser]; ty_wf_E := Euser |} in
     (∀ κ1 κ2, (T κ1).(ty_size) = (T κ2).(ty_size)) →
     (∀ E L κ1 κ2, lctx_lft_eq E L κ1 κ2 → subtype E L (T κ1) (T κ2)) →
@@ -58,12 +81,13 @@ Section diverging_static.
     typed_val (diverging_static_loop call_once)
               (fn(∀ α, ∅; T α, F) → ∅).
   Proof.
-    intros HWf HTsz HTsub Hf E L. iApply type_fn; [solve_typing..|]. iIntros "/= !#".
+    intros type_equivalize_lft_static_bad HWf HTsz HTsub Hf E L.
+    iApply type_fn; [solve_typing..|]. iIntros "/= !#".
       iIntros (α ϝ ret arg). inv_vec arg=>x f. simpl_subst.
     iApply type_let; [apply Hf|solve_typing|]. iIntros (call); simpl_subst.
     iApply (type_cont [_] [] (λ r, [(r!!!0%fin:val) ◁ box (unit)])).
     { iIntros (k). simpl_subst.
-      iApply type_equivalize_lft_static.
+      iApply type_equivalize_lft_static_bad.
       iApply (type_call [ϝ] ()); solve_typing. }
     iIntros "!# *". inv_vec args=>r. simpl_subst.
     iApply (type_cont [] [] (λ r, [])).
@@ -71,5 +95,4 @@ Section diverging_static.
     iIntros "!# *". inv_vec args. simpl_subst.
     iApply type_jump; solve_typing.
   Qed.
-
 End diverging_static.
