theories/typing/lib/fake_shared.v
@@ -14,9 +14,9 @@ Section fake_shared.
   Proof.
     intros E L. iApply type_fn; [solve_typing..|]. iIntros "/= !#".
       iIntros ([α β] ϝ ret arg). inv_vec arg=>x. simpl_subst.
-    iIntros (tid) "#LFT #HE Hna HL Hk HT".
+    iIntros (tid qmax) "#LFT #HE Hna HL Hk HT".
     rewrite tctx_interp_singleton tctx_hasty_val.
-    iDestruct (lctx_lft_incl_incl α β with "HL HE") as "#Hαβ"; [solve_typing..|].
+    iDestruct (lctx_lft_incl_incl α β with "HL HE") as "%"; [solve_typing..|].
     iAssert (▷ ty_own (own_ptr 1 (&shr{α}(box ty))) tid [x])%I with "[HT]" as "HT".
     { destruct x as [[|l|]|]=>//=. iDestruct "HT" as "[H $]".
       iNext. iDestruct "H" as ([|[[]|][]]) "[H↦ H]"; try done.
@@ -25,7 +25,8 @@ Section fake_shared.
       { iApply frac_bor_iff; last done. iIntros "!>!# *".
         rewrite heap_mapsto_vec_singleton. iSplit; auto. }
       iDestruct "H" as "#H". iIntros "!# * % $". iApply step_fupd_intro. set_solver.
-      simpl. by iApply ty_shr_mono. }
+      simpl. iApply ty_shr_mono; last done.
+      by iApply lft_incl_syn_sem. }
     do 2 wp_seq.
     iApply (type_type [] _ _ [ x ◁ box (&shr{α}(box ty)) ]
             with "[] LFT [] Hna HL Hk [HT]"); last first.
@@ -43,9 +44,9 @@ Section fake_shared.
   Proof.
     intros E L. iApply type_fn; [solve_typing..|]. iIntros "/= !#".
       iIntros ([α β] ϝ ret arg). inv_vec arg=>x. simpl_subst.
-    iIntros (tid) "#LFT #HE Hna HL Hk HT".
+    iIntros (tid qmax) "#LFT #HE Hna HL Hk HT".
     rewrite tctx_interp_singleton tctx_hasty_val.
-    iDestruct (lctx_lft_incl_incl α β with "HL HE") as "#Hαβ"; [solve_typing..|].
+    iDestruct (lctx_lft_incl_incl α β with "HL HE") as "%"; [solve_typing..|].
     (* FIXME: WTF, using &uniq{β} here does not work. *)
     iAssert (▷ ty_own (own_ptr 1 (&shr{α} (uniq_bor β ty))) tid [x])%I with "[HT]" as "HT".
     { destruct x as [[|l|]|]=>//=. iDestruct "HT" as "[H $]".
@@ -55,7 +56,9 @@ Section fake_shared.
       { iApply frac_bor_iff; last done. iIntros "!>!# *".
         rewrite heap_mapsto_vec_singleton. iSplit; auto. }
       iDestruct "H" as "#H". iIntros "!# * % $". iApply step_fupd_intro. set_solver.
-      simpl. iApply ty_shr_mono; last done. iApply lft_intersect_incl_l. }
+      simpl. iApply ty_shr_mono; last done.
+      by iApply lft_intersect_incl_l.
+    }
     do 2 wp_seq.
     iApply (type_type [] _ _ [ x ◁ box (&shr{α}(&uniq{β} ty)) ]
             with "[] LFT [] Hna HL Hk [HT]"); last first.
